theories/Logic/PeanoArithmetic.v
@@ -1,0 +1,123 @@
+Require Import Coq.Arith.Compare_dec.
+Require Import Coq.Arith.PeanoNat.
+Require Import Coq.Bool.Bool.
+Require Import Coq.Classes.RelationClasses.
+Require Import Coq.Lists.List.
+Require Import Coq.micromega.Lia.
+Require Import Coq.Program.Basics.
+Require Import Coq.Relations.Relation_Definitions.
+Require Import Coq.Relations.Relation_Operators.
+Require Import DschingisKhan.Prelude.PreludeInit.
+Require Import DschingisKhan.Prelude.PreludeMath.
+Require Import DschingisKhan.Prelude.PreludeUtil.
+Require Import DschingisKhan.Prelude.PreludeClassic.
+
+Module PeanoArithmetic.
+
+  Import ListNotations.
+
+  Definition ivar : Set := nat.
+
+  Inductive term : Set :=
+  | IVarT (x : ivar) : term
+  | ZeroT : term
+  | SuccT (t1 : term) : term
+  | PlusT (t1 : term) (t2 : term) : term
+  | MultT (t1 : term) (t2 : term) : term
+  .
+
+  Inductive formula : Set :=
+  | EqnF (t1 : term) (t2 : term) : formula
+  | LeqF (t1 : term) (t2 : term) : formula
+  | NegF (f1 : formula) : formula
+  | ImpF (f1 : formula) (f2 : formula) : formula
+  | AllF (y : ivar) (f1 : formula) : formula
+  .
+
+  Section SEMANTICS.
+
+  Let universe_of_discourse : Set := nat.
+
+  Let value_assignment : Set := ivar -> universe_of_discourse.
+
+  Fixpoint eval_term (env : value_assignment) (t : term) {struct t} : universe_of_discourse :=
+    match t with
+    | IVarT x => env x
+    | ZeroT => O
+    | SuccT t1 => S (eval_term env t1)
+    | PlusT t1 t2 => eval_term env t1 + eval_term env t2
+    | MultT t1 t2 => eval_term env t1 * eval_term env t2
+    end
+  .
+
+  Fixpoint eval_formula (env : value_assignment) (f : formula) {struct f} : Prop :=
+    match f with
+    | EqnF t1 t2 => eval_term env t1 = eval_term env t2
+    | LeqF t1 t2 => eval_term env t1 <= eval_term env t2
+    | NegF f1 => ~ eval_formula env f1
+    | ImpF f1 f2 => eval_formula env f1 -> eval_formula env f2
+    | AllF y f1 => forall n : universe_of_discourse, eval_formula (fun z : ivar => if eq_dec y z then n else env z) f1
+    end
+  .
+
+  End SEMANTICS.
+
+  Section SUBSTITUTION.
+
+  Definition Subst : Set := ivar -> term.
+
+  Definition nilSubst : Subst :=
+    fun z : ivar => IVarT z
+  .
+
+  Definition consSubst (y : ivar) (t : term) (sigma : Subst) : Subst :=
+    fun z : ivar => if eq_dec y z then t else sigma z
+  .
+
+  Fixpoint fvs_term (t : term) {struct t} : list ivar :=
+    match t with
+    | IVarT x => [x]
+    | ZeroT => []
+    | SuccT t1 => fvs_term t1
+    | PlusT t1 t2 => fvs_term t1 ++ fvs_term t2
+    | MultT t1 t2 => fvs_term t1 ++ fvs_term t2
+    end
+  .
+
+  Fixpoint fvs_formula (f : formula) {struct f} : list ivar :=
+    match f with
+    | EqnF t1 t2 => fvs_term t1 ++ fvs_term t2
+    | LeqF t1 t2 => fvs_term t1 ++ fvs_term t2
+    | NegF f1 => fvs_formula f1
+    | ImpF f1 f2 => fvs_formula f1 ++ fvs_formula f2
+    | AllF y f1 => remove eq_dec y (fvs_formula f1)
+    end
+  .
+
+  Definition chi (sigma : Subst) (f : formula) : ivar :=
+    suc (maxs (map (fun z : ivar => maxs (fvs_term (sigma z))) (fvs_formula f)))
+  .
+
+  Fixpoint subst_term (sigma : Subst) (t : term) {struct t} : term :=
+    match t with
+    | IVarT x => sigma x
+    | ZeroT => ZeroT
+    | SuccT t1 => SuccT (subst_term sigma t1)
+    | PlusT t1 t2 => PlusT (subst_term sigma t1) (subst_term sigma t2)
+    | MultT t1 t2 => MultT (subst_term sigma t1) (subst_term sigma t2)
+    end
+  .
+
+  Fixpoint subst_formula (sigma : Subst) (f : formula) {struct f} : formula :=
+    match f with
+    | EqnF t1 t2 => EqnF (subst_term sigma t1) (subst_term sigma t2)
+    | LeqF t1 t2 => LeqF (subst_term sigma t1) (subst_term sigma t2)
+    | NegF f1 => NegF (subst_formula sigma f1)
+    | ImpF f1 f2 => ImpF (subst_formula sigma f1) (subst_formula sigma f2)
+    | AllF y f1 => let z := chi sigma f in AllF z (subst_formula (consSubst y (IVarT z) sigma) f1)
+    end
+  .
+
+  End SUBSTITUTION.
+
+End PeanoArithmetic.
